{
 "cells": [
  {
   "cell_type": "markdown",
   "metadata": {},
   "source": [
    "# Question.1"
   ]
  },
  {
   "cell_type": "markdown",
   "metadata": {},
   "source": [
    "## (i)\n",
    "Using lagrange multiplier,\n",
    "$$\n",
    "min - \\sum \\log x_i, \\quad \\text{s.t.} \\Sigma x_i = 1\n",
    "$$\n",
    "Denote \n",
    "$$\n",
    "L = - \\sum \\log x_i + \\lambda(\\Sigma x_i - 1)\n",
    "$$\n",
    "Apply F.O.C\n",
    "\n",
    "$$\n",
    "\\frac{\\partial L}{\\partial x_i} = 0 \\Rightarrow -\\frac{1}{x_i} + \\lambda = 0 \\Rightarrow x_i = \\frac 1\\lambda\n",
    "$$\n",
    "$$\n",
    "\\frac{\\partial L}{\\partial \\lambda} = 0 \\Rightarrow \\Sigma x_i = 1 \\Rightarrow x_i = \\frac 1n, \\lambda = n\n",
    "$$"
   ]
  },
  {
   "cell_type": "markdown",
   "metadata": {},
   "source": [
    "## (ii)\n",
    "Similar to (i), denote that \n",
    "$$\n",
    "L = -\\sum\\log x_i + (Ax - b)^T\\lambda\n",
    "$$\n",
    "Apply F.O.C,\n",
    "\n",
    "Here, $A_{ji}$ is the jth row, ith col element in A.\n",
    "$$\n",
    "\\frac{\\partial L}{\\partial x_i} = 0 \\Rightarrow  -\\frac{1}{x_i} + \\lambda\\sum_j A_{ji} = 0\n",
    "$$\n",
    "$$\n",
    "\\frac{\\partial L}{\\partial\\lambda} = 0 \\Rightarrow Ax = b.\n",
    "$$\n",
    "From the first equaiton, we find that \n",
    "$$x_i = \\frac{1}{\\lambda\\sum_jA_{ji}} = \\frac{1}{(A^T\\lambda)_i}$$.\n",
    "\n",
    "Also we have,\n",
    "$$Ax = \n",
    "A\\left(\\begin{array}{c}\\frac{1}{\\lambda \\sum_j A_{j1}}\\\\\n",
    "\\vdots\\\\\n",
    "\\frac{1}{\\lambda \\sum_j A_{jn}}\\\\\n",
    "\\end{array}\\right) = \n",
    "\\left(\n",
    "\\begin{array}{c}\\sum_i\\frac{ A_{1i}}{\\lambda \\sum_j A_{ji}}\\\\\n",
    "\\vdots\\\\\n",
    "\\sum_i\\frac{ A_{ni}}{\\lambda \\sum_j A_{ji}}\\\\\n",
    "\\end{array}\\right)\n",
    "$$\n",
    "Thus we have\n",
    "$$\n",
    "x^TA^T \\lambda = \\left(\n",
    "\\begin{array}{c}\\sum_i\\frac{ A_{1i}}{\\lambda \\sum_j A_{ji}}&\n",
    "\\cdots&\n",
    "\\sum_i\\frac{ A_{ni}}{\\lambda \\sum_j A_{ji}}\\\\\n",
    "\\end{array}\\right)\n",
    "\\left(\\begin{array}{cc}\\lambda\\\\ \n",
    "\\vdots\\\\\n",
    "\\lambda \\end{array}\\right) = n\n",
    "$$\n",
    "Thus we get the dual larange function\n",
    "$$\n",
    "q(\\lambda) = \\inf_{\\lambda}( -\\sum\\log x_i + (Ax - b)^T\\lambda) = -b^T\\lambda - \\sum_{i = 1}^{n} \\frac{1}{(A^T\\lambda)_i} + n\n",
    "$$\n",
    "i.e.\n",
    "$$\n",
    "\\max q(\\lambda) = -b^T\\lambda +\\sum_{i = 1}^{n} {(A^T\\lambda)_i} + n\\qquad \\text{where } \\lambda > 0.\n",
    "$$\n",
    "\n",
    "This is the dual problem.\n"
   ]
  },
  {
   "cell_type": "markdown",
   "metadata": {},
   "source": [
    "## (iii)\n",
    "Already solved in (ii)"
   ]
  },
  {
   "cell_type": "markdown",
   "metadata": {},
   "source": [
    "## (iv)\n",
    "By newton's method, we need to calculate the matrix equation\n",
    "$$\n",
    "\\begin{bmatrix}\n",
    "\\nabla^2 f &A^T\\\\\n",
    "A& 0\n",
    "\\end{bmatrix}\n",
    "\\begin{bmatrix}\n",
    "-\\Delta x\\\\\n",
    "\\lambda\n",
    "\\end{bmatrix}\n",
    "=\n",
    "\\begin{bmatrix}\n",
    "-\\nabla f(x)\\\\\n",
    "0\n",
    "\\end{bmatrix}\n",
    "$$\n",
    "It's easy to see that \n",
    "\n",
    "$$\n",
    "\\nabla f = (-\\frac{1}{x_1},\\cdots, -\\frac{1}{x_n})^T\n",
    "$$\n",
    "\n",
    "$$\n",
    "\\nabla^2 f = diag(\\frac{1}{x_1^2},\\cdots, \\frac{1}{x_n^2})\n",
    "$$"
   ]
  },
  {
   "cell_type": "code",
   "execution_count": 166,
   "metadata": {},
   "outputs": [],
   "source": [
    "import numpy as np\n",
    "from numpy.linalg import inv\n",
    "def NewtonMethod_acp(A, x0, alpha, beta, tol):\n",
    "    def decrement(dfx, H):\n",
    "        # define the function to calculate lambda(x), which is the Newton decrement\n",
    "        return np.sqrt(np.dot(dfx.T,np.dot(np.diag(1/np.diag(H)), dfx)))\n",
    "    (row, col) = A.shape\n",
    "    x = x0\n",
    "    H = np.diag(x) # H is hessian of f(x)\n",
    "    upper = np.column_stack((H, A.T)) # [Hessian, A^T]\n",
    "    lower = np.column_stack((A, np.zeros((row, row)))) # [A, 0]\n",
    "    KKT = np.row_stack((upper, lower)) # this the the matrix on the left\n",
    "    dfx = 1 / x # this is - nabla f(x)\n",
    "    RHS = np.append(dfx, np.zeros(row)) # right hand side\n",
    "    epsilon =  decrement(dfx, H) # get the Newton decrement\n",
    "    count = 0\n",
    "    while epsilon > tol and count < 50:\n",
    "        count = count + 1\n",
    "        LHS = np.squeeze(np.array(inv(KKT).dot(RHS)))\n",
    "        dx = np.array(LHS)[:col]\n",
    "        t = 1\n",
    "        print (x)\n",
    "        # using backtracking line search\n",
    "        while -np.log(x + t * dx).sum() >= -np.log(x).sum() - alpha * t * dfx.T.dot(dx):\n",
    "            t = t * beta\n",
    "        print (t)\n",
    "        # update the parameters\n",
    "        x = x + t * dx\n",
    "        H = np.diag(x)\n",
    "        upper = np.column_stack((H, A.T))\n",
    "        lower = np.column_stack((A, np.zeros((row, row))))\n",
    "        KKT = np.row_stack((upper, lower))\n",
    "        dfx = 1 / x\n",
    "        RHS = np.append(dfx, np.zeros(row))\n",
    "        epsilon =  decrement(dfx, H)\n",
    "    return x"
   ]
  },
  {
   "cell_type": "code",
   "execution_count": 43,
   "metadata": {},
   "outputs": [],
   "source": [
    "A = np.matrix([1,1,1])"
   ]
  },
  {
   "cell_type": "code",
   "execution_count": 164,
   "metadata": {},
   "outputs": [],
   "source": [
    "x0 = np.array([0.5,0.9,1])"
   ]
  },
  {
   "cell_type": "code",
   "execution_count": 50,
   "metadata": {},
   "outputs": [],
   "source": [
    "a = 0.1\n",
    "b = 0.5\n",
    "tol = 0.00001"
   ]
  },
  {
   "cell_type": "code",
   "execution_count": 168,
   "metadata": {},
   "outputs": [
    {
     "data": {
      "text/plain": [
       "array([-0.51337591,  2.02675183, -0.51337591])"
      ]
     },
     "execution_count": 168,
     "metadata": {},
     "output_type": "execute_result"
    }
   ],
   "source": [
    "res"
   ]
  },
  {
   "cell_type": "markdown",
   "metadata": {},
   "source": [
    "# Question.2"
   ]
  },
  {
   "cell_type": "markdown",
   "metadata": {},
   "source": [
    "## (a)\n",
    "\n",
    "First, show the equivelent between these 4 conditions.\n",
    "___\n",
    "* Condition 1 is equivalent to Condition 2\n",
    "\n",
    "Condition 1 $\\rightarrow$ Condition 2\n",
    "\n",
    "Suppose $x \\in \\mathcal N(A) \\cap \\mathcal N(H)$ and $x \\neq 0$. In condition 2, we have  $Ax = 0\\, x \\neq 0$. Since $x \\in \\mathcal N(A) \\cap \\mathcal N(H)$, we have $x^THx = 0$, this contradict to to second statement.\n",
    "\n",
    "Condition 2 $\\rightarrow$ Condition 1\n",
    "\n",
    "If there is an $x$ s.t. $Ax = 0\\, x \\neq 0, x^THX = 0$. Because $H$ is semipositive definate, we must have $Hx = 0$, i.e.   $x \\in \\mathcal N(A) \\cap \\mathcal N(H)$\n",
    "___\n",
    "* Condition 2 is equivalent to Condition 3\n",
    "\n",
    "If $Ax = 0, x \\neq 0$, then because $\\mathcal R(F) = \\mathcal N (A)$, we have $x = Fz$ and $z \\neq 0$. Then because of 2 we have $x^T Hx = z^TF^THFZ > 0$\n",
    "\n",
    "___\n",
    "* Condition 2 is equivalent to Condition 4\n",
    "If we have the condition 2. then \n",
    "\n",
    "$$\n",
    "x^T(H + A^TA) = x^THx + \\vert\\vert A^Tx\\vert\\vert^2_2 > 0\n",
    "$$\n",
    "for all nonzero x, sot the condition 4 holds for $Q = I$.\n",
    "If the fourth condition hols with general semipositive definate form of $Q$.\n",
    "$$\n",
    "x^T(H + A^TQA) = x^THx + x^TA^TQAx > 0\n",
    "$$\n",
    "for all nonzero $x$, Therefore if $Ax = 0\\, x \\neq 0$, we must have $x\\neq 0$\n",
    "___\n",
    "Second show these four conditions are equivalent to nonsigularity of KKT matrix.\n",
    "\n",
    "Suppose $x\\neq 0$, s.t.$Ax = 0, Hx = 0$\n",
    "$$\n",
    "\\begin{bmatrix}\n",
    "H & A^T\\\\\n",
    "A & 0\n",
    "\\end{bmatrix}\n",
    "\\begin{bmatrix}\n",
    "x\\\\\n",
    "0\n",
    "\\end{bmatrix} = 0$$\n",
    "\n",
    "If the KKT matrix is singular, $x,z$ are not both zero, and we have\n",
    "$$\n",
    "\\begin{bmatrix}\n",
    "H & A^T\\\\\n",
    "A & 0\n",
    "\\end{bmatrix}\n",
    "\\begin{bmatrix}\n",
    "x\\\\\n",
    "z\n",
    "\\end{bmatrix} = 0$$\n",
    "\n",
    "This leads to $Hx + A^Tz = 0$, and $Ax = 0$. \n",
    "from the first equation, we have \n",
    "$$\n",
    "x^THx + x^TA^Tz = 0.\n",
    "$$\n",
    "plug in the second equation.\n",
    "we have $x^THx = 0$, this contradicts second condition unless $x= 0$.\n",
    "\n",
    "## (b)\n",
    "From previous question, we have $H + A^TA$ is positive definate matrix. Then we must hvae $R \\in \\mathbb R^{n\\times n}$, s.t.\n",
    "$$\n",
    "R^T(H + A^TA)R = I\n",
    "$$\n",
    "Apply SVD to $AR$, $AR = U\\Sigma V_1^T$, where $\\Sigma = diag(\\sigma_1,\\cdots, \\sigma_p)$. Denote $V_2 \\in \\mathbb R^{n\\times(n-p)}$, s.t.\n",
    "$$\n",
    "V = \\left[V_1\\quad V_2\\right]\n",
    "$$\n",
    "$V_2$ is orthogonal, and let \n",
    "$$\n",
    "S = \\left[\\Sigma\\quad 0\\right] \\in \\mathbb R^{p\\times n}\n",
    "$$\n",
    "We have $AR = USV^T$, then \n",
    "$$\n",
    "V^TR^T(H + A^TA)RV = V^TR^THRV + S^TS = I\n",
    "$$\n",
    "Becasue $V^TR^THRV = I - S^TS$ is diagonal matrix, then denote it as $D$\n",
    "$$\n",
    "D = V^TR^THRV = diag(1-\\sigma_1^2, \\cdots, 1-\\sigma_p^2, 1, \\cdots, 1)\n",
    "$$\n",
    "Apply the transform to KKT matrix, we have\n",
    "\n",
    "$$\n",
    "\\begin{bmatrix}\n",
    "V^TR^T & 0\\\\\n",
    "0 & U\n",
    "\\end{bmatrix}\n",
    "\\begin{bmatrix}\n",
    "H & A^T\\\\\n",
    "A & 0\n",
    "\\end{bmatrix}\n",
    "\\begin{bmatrix}\n",
    "RV & 0\\\\\n",
    "0 & U\n",
    "\\end{bmatrix}\n",
    "=\n",
    "\\begin{bmatrix}\n",
    "D & S^T\\\\\n",
    "S & 0\n",
    "\\end{bmatrix}\n",
    "$$\n",
    "Apply the permutation to hte matrix on the right gives a block diaonal matrix with n diagonal blocks.\n",
    "$$\n",
    "\\begin{bmatrix}\n",
    "\\lambda_i & \\sigma_i\\\\\n",
    "\\sigma_i & 0\n",
    "\\end{bmatrix}\n",
    "$$\n",
    "where $i = 1,2,\\cdots, p$, \n",
    "\n",
    "and $\\lambda_i = 1$ for $i = p +1, \\cdots, n$\n",
    "\n",
    "This matrix have eiggenvalues of $\\frac{\\lambda_i \\pm \\sqrt{\\lambda_i^2 + 4\\sigma_i^2}}{2}$, i.e. one eigen value is positive, another is negative. \n",
    "\n",
    "In total, there are n positive evalues and p negative evalues."
   ]
  }
 ],
 "metadata": {
  "kernelspec": {
   "display_name": "Python 3",
   "language": "python",
   "name": "python3"
  },
  "language_info": {
   "codemirror_mode": {
    "name": "ipython",
    "version": 3
   },
   "file_extension": ".py",
   "mimetype": "text/x-python",
   "name": "python",
   "nbconvert_exporter": "python",
   "pygments_lexer": "ipython3",
   "version": "3.6.4"
  }
 },
 "nbformat": 4,
 "nbformat_minor": 2
}
