\documentclass[a4paper]{article}

%% Language and font encodings
\usepackage[english]{babel}
\usepackage[utf8x]{inputenc}
\usepackage[T1]{fontenc}

%% Sets page size and margins
\usepackage[a4paper,top=3cm,bottom=2cm,left=3cm,right=3cm,marginparwidth=1.75cm]{geometry}

%% Useful packages
\usepackage{amsmath}
\usepackage{graphicx}
\usepackage[colorinlistoftodos]{todonotes}
\usepackage{mathrsfs}
\usepackage{amsfonts,amssymb}
\usepackage[colorlinks=true, allcolors=blue]{hyperref}

\title{Homework 2}
\author{Yang Li, Jimmy Jusuf, Zhirong Zhang, Tiangang Zhang }

\begin{document}
\maketitle


\section{Problem 1}
\begin{eqnarray*}
L(x,\lambda)=(x-a)^2+(y-b)^2-\lambda_1 x+\lambda_2 (x-1)-\lambda_3 y +\lambda_4 (y-1)
\end{eqnarray*}
Then local minimizer should subject to

\begin{equation}  
\left\{  
             \begin{array}{ll}
             2(x^*-a)-\lambda_1^*+\lambda_2^*=0\\  
             2(y^*-a)-\lambda_3^*+\lambda_4^*=0\\
             \lambda_1^* x^*=0\\
             \lambda_2^*(x^*-1)=0\\
             \lambda_3^* y^*=0\\
             \lambda_4^*(y^*-1)=0\\
             \lambda_i^* \geq 0 & for \,  i=1,2,3,4
             \end{array}  
\right.  
\end{equation}  

Solve the equations above, the solution is
\begin{equation}  
x^*=
\left\{  
             \begin{array}{ll}
             0 & a\leq 0\\
             a & a \in (0,1) \\
             1 & a \geq 1
             \end{array}  
\right.  
\end{equation} 
\begin{equation}  
y^*=
\left\{  
             \begin{array}{ll}
             0 & b\leq 0\\
             b & b \in (0,1) \\
             1 & b \geq 1
             \end{array}  
\right.  
\end{equation}  

\section{Problem 2}
Let $x_2-10=x^+-x^-,\, x^+,x^-\geq 0$, use the property of absolute value inequalities, the problem become
\begin{equation}  
min \, 2x_1+3|x^+-x^-|, \text{ subject to}
\left\{  
             \begin{array}{ll}
             x_1+2+10+x^+-x^-\leq 5\\
             -x_1-2+10+x^+-x^-\leq 5\\
             x_1+2-10-x^++x^-\leq 5\\
             -x_1-2-10-x^++x^-\leq 5\\
             x^+,x^-\geq 0
             \end{array}  
\right.  
\end{equation}  

Notice that 
\begin{equation}  
2x_1+3(x^++x^-) \geq 2x_1+3|x^+-x^-|
\end{equation}  
now we consider 
\begin{equation}  
min \,2x_1+3(x^++x^-) , \text{ subject to}
\left\{  
             \begin{array}{ll}
             x_1+2+10+x^+-x^-\leq 5\\
             -x_1-2+10+x^+-x^-\leq 5\\
             x_1+2-10-x^++x^-\leq 5\\
             -x_1-2-10-x^++x^-\leq 5\\
             x^+,x^-\geq 0
             \end{array}  
\right.  
\end{equation}  
Let $x_1^*,x^{+*},x^{-*}$ be the minimizer of the problem above, the next step is to prove that  $x_1^*,x^{+*},x^{-*}$ is the minimizer of the original problem, we prove by contradiction.
If there is $x_1',x_2'$ subject to the conditions and 
\begin{equation}  
2x_1'^*+3|x_2'-10| < 2x_1^*+3(x^{+*}+x^{+*})
\end{equation}  
Let 
\begin{eqnarray*}  
x_{1\star}=x_1'\\
x^{+}_\star=\{x_2'-10\}^+\\
x^{^-}_\star=\{-x_2'+10\}^+
\end{eqnarray*}  
Then 
\begin{equation}  
2x_{1\star}+3(x^{+}_\star+x^{^-}_\star) < 2x_1^*+3(x^{+*}+x^{+*})
\end{equation}  
Contradition!

Recall equation(5) we know that
\begin{equation}  
2x_1'^*+3|x_2'-10| = 2x_1^*+3(x^{+*}+x^{+*})
\end{equation}  
So we can always use the minimizer of problem (6) to get the minimizer and minimum value of the original problem. Then problem has been transfered into a LP
\begin{equation}  
min \,2x_1+3(x^++x^-) , \text{ subject to}
\left\{  
             \begin{array}{ll}
             x_1+2+10+x^+-x^-\leq 5\\
             -x_1-2+10+x^+-x^-\leq 5\\
             x_1+2-10-x^++x^-\leq 5\\
             -x_1-2-10-x^++x^-\leq 5\\
             x^+,x^-\geq 0
             \end{array}  
\right.  
\end{equation}  

\section{Problem 3}
According to no-arbitrage condition, there is no need to trade a currency back to the currency it traded from. The trade from one currency to another currency happens at most for one time. So we can write the problem as 
\begin{equation}  
max \,\sum_{i \not= N} f_{iN} x_{iN}, \text{ subject to}
\left\{  
             \begin{array}{ll}
             \sum_{j\not= 1}x_{1j}\leq B,\\
             \sum_{j\not= 1}x_{1j}\leq u_1,\\
             \sum_{j\not= 1, i}x_{ij}\leq \sum_{k\not=i,N}f_{ki} x_{ki},& for\, i\not= 1,N\\
             \sum_{j\not= 1, i}x_{ij}\leq u_i,& for\, i\not= 1,N\\
             x_{ij}\geq 0, & for\, i\not= j,i\not=N
             \end{array}  
\right.  
\end{equation}  
\end{document}